RS_Init

ironfleet/ravana/DistributedSystem.i.dfy
@@ -1,19 +1,35 @@
 include "Node.i.dfy"
 include "Types.i.dfy"
+include "../src/Dafny/Distributed/Impl/Common/SeqIsUniqueDef.i.dfy"
 
 module DistributedSystem_i {
+  import opened Types_i
   import opened Protocol_Node_i
+  import opened Common__SeqIsUniqueDef_i
 
-  predicate RS_Init(rs: RS_State, config: Config)
+  predicate RS_Init(rs: RState, config: Config)
   {
-       LEnvironment_Init(rs.environment)
+       LEnvironment_Init(rs.env)
+
+    && NodeInit_Logger(rs.server_logger, config)
+
+    && SeqIsUnique([config.node_logger] + config.node_controllers + config.node_switches)
+
     && |config.node_controllers| > 0
+    && (forall e :: e in rs.server_controllers <==> e in config.node_controllers)
+    && (forall index :: 0 <= index < |config.node_controllers| ==>
+            NodeInit_Controller(rs.server_controllers[config.node_controllers[index]],
+                                index,
+                                config)
+       )
+
     && |config.node_switches| > 0
-    && NodeInit_Logger(config.node_logger, config)
-    && (forall e :: e in rs.servers <==> (e == config.node_logger
-          || e in config.node_controllers || e in config.node_switches))
-    && NodeInit_Controller(rs.servers[config.node_logger], config)
-    && (forall e in config.node_controllers ::
-          NodeInit_Logger
+    && (forall e :: e in rs.server_switches <==> e in config.node_switches)
+    && (forall index :: 0 <= index < |config.node_switches| ==>
+            NodeInit_Switch(rs.server_switches[config.node_switches[index]],
+                           index,
+                           config)
+       )
+
   }
 }
